isabelle/elaborator/ElabType.thy
@@ -2,19 +2,19 @@ theory ElabType
   imports TypeError Typedefs "../core/CoreTyEnv" "../util/NatToString" "../util/DistinctCheck"
 begin
 
-(* Input: env, typedefs, ghost mode, input type (or list) *)
+(* Input: env, elabEnv, ghost mode, input type (or list) *)
 (* Output: either a list of errors, or an elaborated type (or list) *)
 
-fun elab_type :: "CoreTyEnv \<Rightarrow> Typedefs \<Rightarrow> GhostOrNot \<Rightarrow> BabType
+fun elab_type :: "CoreTyEnv \<Rightarrow> ElabEnv \<Rightarrow> GhostOrNot \<Rightarrow> BabType
                   \<Rightarrow> TypeError list + CoreType"
-and elab_type_list :: "CoreTyEnv \<Rightarrow> Typedefs \<Rightarrow> GhostOrNot \<Rightarrow> BabType list
+and elab_type_list :: "CoreTyEnv \<Rightarrow> ElabEnv \<Rightarrow> GhostOrNot \<Rightarrow> BabType list
                       \<Rightarrow> TypeError list + CoreType list"
 where
-  "elab_type env typedefs ghost (BabTy_Name loc name tyargs) =
-    (case elab_type_list env typedefs ghost tyargs of
+  "elab_type env elabEnv ghost (BabTy_Name loc name tyargs) =
+    (case elab_type_list env elabEnv ghost tyargs of
       Inl errs \<Rightarrow> Inl errs
     | Inr elabTyArgs \<Rightarrow>
-        (case fmlookup typedefs name of
+        (case fmlookup (EE_Typedefs elabEnv) name of
           Some (tyvars, targetTy) \<Rightarrow>
             \<comment> \<open>Typedef case (also handles type variables, which map to CoreTy_Var)\<close>
             (if length elabTyArgs \<noteq> length tyvars then
@@ -41,48 +41,48 @@ where
                 \<comment> \<open>Unknown type name\<close>
                 Inl [TyErr_UnknownTypeName loc name])))"
 
-| "elab_type env typedefs ghost (BabTy_Bool loc) =
+| "elab_type env elabEnv ghost (BabTy_Bool loc) =
     Inr CoreTy_Bool"
 
-| "elab_type env typedefs ghost (BabTy_FiniteInt loc sign bits) =
+| "elab_type env elabEnv ghost (BabTy_FiniteInt loc sign bits) =
     Inr (CoreTy_FiniteInt sign bits)"
 
-| "elab_type env typedefs ghost (BabTy_MathInt loc) =
+| "elab_type env elabEnv ghost (BabTy_MathInt loc) =
     (if ghost = NotGhost then
       Inl [TyErr_NonRuntimeType loc]
     else
       Inr CoreTy_MathInt)"
 
-| "elab_type env typedefs ghost (BabTy_MathReal loc) =
+| "elab_type env elabEnv ghost (BabTy_MathReal loc) =
     (if ghost = NotGhost then
       Inl [TyErr_NonRuntimeType loc]
     else
       Inr CoreTy_MathReal)"
 
-| "elab_type env typedefs ghost (BabTy_Tuple loc types) =
-    (case elab_type_list env typedefs ghost types of
+| "elab_type env elabEnv ghost (BabTy_Tuple loc types) =
+    (case elab_type_list env elabEnv ghost types of
       Inl errs \<Rightarrow> Inl errs
     | Inr elabTys \<Rightarrow> Inr (CoreTy_Record (zip (tuple_field_names (length elabTys)) elabTys)))"
 
   (* The Record case preserves field names *)
-| "elab_type env typedefs ghost (BabTy_Record loc flds) =
+| "elab_type env elabEnv ghost (BabTy_Record loc flds) =
     (case first_duplicate_name fst flds of
       Some dupName \<Rightarrow> Inl [TyErr_DuplicateFieldName loc dupName]
     | None \<Rightarrow>
-        (case elab_type_list env typedefs ghost (map snd flds) of
+        (case elab_type_list env elabEnv ghost (map snd flds) of
           Inl errs \<Rightarrow> Inl errs
         | Inr elabTys \<Rightarrow> Inr (CoreTy_Record (zip (map fst flds) elabTys))))"
 
   (* Array case TODO (as we may have to evaluate constants which we can't do yet) 
      Just elaborate to Bool for now *)
-| "elab_type env typedefs ghost (BabTy_Array loc elemTy dims) =
+| "elab_type env elabEnv ghost (BabTy_Array loc elemTy dims) =
     Inr CoreTy_Bool"
 
-| "elab_type_list env typedefs ghost [] = Inr []"
+| "elab_type_list env elabEnv ghost [] = Inr []"
 
-| "elab_type_list env typedefs ghost (ty # tys) =
-    (case (elab_type env typedefs ghost ty,
-           elab_type_list env typedefs ghost tys) of
+| "elab_type_list env elabEnv ghost (ty # tys) =
+    (case (elab_type env elabEnv ghost ty,
+           elab_type_list env elabEnv ghost tys) of
       (Inl errs1, Inl errs2) \<Rightarrow> Inl (errs1 @ errs2)
     | (Inl errs, Inr _) \<Rightarrow> Inl errs
     | (Inr _, Inl errs) \<Rightarrow> Inl errs
