isabelle/elaborator/Typedefs.thy
@@ -18,4 +18,23 @@ definition typedefs_well_formed :: "CoreTyEnv \<Rightarrow> Typedefs \<Rightarro
         is_well_kinded env targetTy \<and>
         type_tyvars targetTy \<subseteq> set tyvars)"
 
+(* The elaborator environment extends the core type environment with
+   information that only the elaborator needs:
+   - Babylon-level typedefs (resolved to their underlying types before entering Core)
+   - The set of nullary data constructor names (Core doesn't track this) *)
+record ElabEnv =
+  EE_Typedefs :: Typedefs
+  EE_NullaryDataCtors :: "string fset"
+
+(* Well-formedness of the elaborator environment:
+   - Typedefs are well-formed
+   - Every nullary data constructor name actually exists in TE_DataCtors
+     with payload type CoreTy_Record [] (the unit type) *)
+definition elabenv_well_formed :: "CoreTyEnv \<Rightarrow> ElabEnv \<Rightarrow> bool" where
+  "elabenv_well_formed env ee =
+    (typedefs_well_formed env (EE_Typedefs ee)
+   \<and> (\<forall>name. name |\<in>| EE_NullaryDataCtors ee \<longrightarrow>
+        (\<exists>dtName tyvars. fmlookup (TE_DataCtors env) name
+                         = Some (dtName, tyvars, CoreTy_Record []))))"
+
 end
